examples/new_echo/NewEcho01proof.v
@@ -1,0 +1,169 @@
+Require Import NewEcho0 NewEcho1 HoareDef SimModSem.
+Require Import NewStack3A.
+Require Import Coqlib.
+Require Import Universe.
+Require Import Skeleton.
+Require Import PCM.
+Require Import ModSem Behavior.
+Require Import Relation_Definitions.
+
+(*** TODO: export these in Coqlib or Universe ***)
+Require Import Relation_Operators.
+Require Import RelationPairs.
+From ITree Require Import
+     Events.MapDefault.
+From ExtLib Require Import
+     Core.RelDec
+     Structures.Maps
+     Data.Map.FMapAList.
+Require Import TODOYJ.
+Require Import HTactics Logic IPM.
+Require Import OpenDef STB.
+
+Set Implicit Arguments.
+
+Local Open Scope nat_scope.
+
+
+
+Section SIMMODSEM.
+
+  Context `{Σ: GRA.t}.
+  Context `{@GRA.inG stkRA Σ}.
+
+  Let W: Type := ((Σ * Any.t)) * ((Σ * Any.t)).
+
+  Let wf: _ -> W -> Prop :=
+    @mk_wf _ unit
+           (fun _ _ _ => ⌜True⌝%I)
+           top4
+  .
+
+  (*** TODO: remove this later ***)
+  Definition ClientStb: list (gname * fspec).
+    eapply (Seal.sealing "stb").
+    let x := constr:(List.map (fun fn => (fn, (KModSem.disclose_tgt fspec_trivial))) ["getint"; "putint"]) in
+    let y := eval cbn in x in
+    eapply y.
+  Defined.
+  (* Global Opaque ClientStb. *)
+  Hint Unfold ClientStb: stb.
+
+  Variable global_stb: list (string * fspec).
+  Hypothesis STBINCL: stb_incl (ClientStb ++ EchoStb ++ StackStb) global_stb.
+
+  Ltac renamer := idtac.
+  Ltac post_call :=
+    fold wf; clear_fast; mDesAll; des_safe; subst; try rewrite Any.upcast_downcast in *; clarify; renamer.
+
+  (* Local Opaque is_int_stack. *)
+  (* Lemma unfold_is_int_stack *)
+  (*       h stk0 *)
+  (*   : *)
+  (*     is_int_stack h stk0 = is_int_stack h stk0 *)
+  (* . *)
+  (* Proof. *)
+  (* Qed. *)
+
+  Theorem sim_modsem: ModSemPair.sim (NewEcho1.EchoSem global_stb) (NewEcho0.EchoSem).
+  Proof.
+    econstructor 1 with (wf:=wf) (le:=top2); ss; et; swap 2 3.
+    { esplits. econs; ss.
+      - eapply to_semantic. iIntros "H". ss.
+    }
+    econs; ss.
+    { unfold NewEcho0.echo_body, echo_body, cfun, kcall, ccall. trivial_init. post_call.
+      des_ifs. steps. unfold KModSem.transl_fun_tgt. steps. rewrite _UNWRAPN. steps.
+      kstart 1. kcatch. { eapply STBINCL. stb_tac; ss. } hcall _ (Some _) _ with ""; ss; et.
+      { ss. }
+      post_call. steps. kstop. steps. erewrite STBINCL; cycle 1. { stb_tac; ss. } steps.
+      hcall _ (Some _) _ with "A"; ss; et.
+      { iModIntro. iSplits; ss; et. }
+      { ss. }
+      post_call. steps. rewrite Any.upcast_downcast. steps.
+      erewrite STBINCL; cycle 1. { stb_tac; ss. } steps.
+      hcall _ (Some _) _ with "A"; ss; et.
+      { iModIntro. iSplits; ss; et. }
+      { ss. }
+      post_call. steps. rewrite Any.upcast_downcast. steps.
+      hret _; ss.
+    }
+    econs; ss.
+    { unfold NewEcho0.input_body, input_body, cfun, kcall, ccall. init. harg. post_call.
+      unfold KModSem.transl_fun_tgt.
+      destruct x; des_ifs_safe; mDesAll; ss; des; subst; cycle 1.
+      { rewrite Any.pair_split. steps. rewrite ! Any.upcast_downcast. steps. }
+      rewrite Any.pair_split. steps. rewrite ! Any.upcast_downcast in *. clarify. steps.
+      erewrite STBINCL; cycle 1. { stb_tac; ss. } steps.
+      hcall _ (Some _) _ with ""; ss; et.
+      post_call. steps. rewrite _UNWRAPN. steps.
+      destruct v; ss; clarify. des_ifs.
+      - steps. hret _; ss.
+        { iModIntro. iSplits; ss; et. }
+      - steps.
+        kstart 1. kcatch.
+        { erewrite STBINCL; ss. stb_tac; ss. }
+        hcall _ (Some (_, _, _)) _ with "-"; ss; et.
+        { iModIntro. iSplits; ss; et. }
+        { ss. }
+        post_call. steps. kstop. steps.
+
+        erewrite STBINCL; cycle 1. { stb_tac; ss. } steps.
+        hcall _ (Some _) _ with "-"; ss; et.
+        { iModIntro. iSplits; ss; et. }
+        { ss. }
+        post_call. steps. rewrite Any.upcast_downcast. steps.
+        hret _; ss.
+        { iModIntro. iSplits; ss; et. }
+    }
+    econs; ss.
+    { unfold NewEcho0.output_body, output_body, cfun, kcall, ccall. init. harg. post_call.
+      unfold KModSem.transl_fun_tgt.
+      destruct x; des_ifs_safe; mDesAll; ss; des; subst; cycle 1.
+      { rewrite Any.pair_split. steps. rewrite ! Any.upcast_downcast. steps. }
+      rewrite Any.pair_split. steps. rewrite ! Any.upcast_downcast in *. clarify. steps.
+      kstart 1. kcatch.
+      { erewrite STBINCL; ss. stb_tac; ss. }
+      hcall _ (Some (_, _)) _ with "-"; ss; et.
+      { iModIntro. iSplits; ss; et. }
+      { ss. }
+      post_call. steps. kstop. steps.
+      destruct a0 as [|hd tl]; ss.
+      - steps. mDesAll; ss; des; subst. rewrite Any.upcast_downcast in *. clarify. steps. hret _; ss.
+        { iModIntro. iSplits; ss; et. }
+      - steps. mDesAll; ss; des; subst. rewrite Any.upcast_downcast in *. clarify.
+        erewrite STBINCL; cycle 1. { stb_tac; ss. } steps.
+        inv PURE0. des_ifs. steps.
+        hcall _ (Some _) _ with ""; ss; et.
+        post_call. steps. rewrite _UNWRAPN. steps.
+        erewrite STBINCL; cycle 1. { stb_tac; ss. } steps.
+        hcall _ (Some _) _ with "-"; ss; et.
+        { iModIntro. iSplits; ss; et. }
+        { ss. }
+        post_call. steps. rewrite Any.upcast_downcast. steps.
+        hret _; ss.
+        { iModIntro. iSplits; ss; et. }
+    }
+  Unshelve.
+    all: ss.
+  Qed.
+
+End SIMMODSEM.
+
+
+
+Section SIMMOD.
+
+  Context `{Σ: GRA.t}.
+  Context `{@GRA.inG stkRA Σ}.
+
+  Variable global_stb: Sk.t -> list (string * fspec).
+  Hypothesis STBINCL: forall sk, stb_incl (ClientStb ++ EchoStb ++ StackStb) (global_stb sk).
+
+  Theorem correct: ModPair.sim (NewEcho1.Echo global_stb) (NewEcho0.Echo).
+  Proof.
+    econs; ss.
+    { ii. eapply sim_modsem; ss. }
+  Qed.
+
+End SIMMOD.
